ver3_less_complex/Thereom.dfy
@@ -1,11 +1,13 @@
 include "Type.dfy"
 include "System.dfy"
 include "Trace.dfy"
+include "Invariants.dfy"
 
 module M_Thereom {
     import opened M_SpecTypes
     import opened M_System
     import opened M_Trace
+    import opened M_Invariants
 
     predicate consistentBlockchains(bc1 : Blockchain, bc2 : Blockchain)
     {
@@ -22,10 +24,50 @@ module M_Thereom {
     }
 
 
-    lemma LemmaBlockchainConsistency(t : Trace, c : Configuration)
-    requires ValidTrace(t, c)
-    ensures consistency(t)
-    {
+    // lemma LemmaBlockchainConsistency(t : Trace, c : Configuration)
+    // requires ValidTrace(t, c)
+    // ensures consistency(t)
+    // {
         
+    // }
+
+    ghost predicate Inv_All(ss : SystemState)
+    {
+        && Inv_Constant_Fields(ss)
+        && Inv_Honest_Node_Only_Vote_One_Proposal_At_Same_View(ss)
+        && Inv_Honest_Node_Only_Vote_One_Prepare_At_Same_View(ss)
+        && Inv_Honest_Node_Only_Vote_One_PreCommit_At_Same_View(ss)
     }
+
+    /**
+     * Here we conduct our safety proof by 3 steps:
+     * Step 1 : Initial system state holds invariants.
+     * Step 2 : All system transition holds invariants as well.
+     * Step 3 : These invariants imply the safety property.
+     */
+
+    lemma Lemma_Initial_State_Holds_Inv(ss : SystemState)
+    requires SystemInit(ss, ss.configuration)
+    ensures Inv_All(ss)
+    {}
+
+
+    lemma Lemma_State_Transition_Holds_Inv(ss : SystemState, ss' : SystemState)
+    requires SystemNext(ss, ss')
+    ensures Inv_All(ss) && Inv_All(ss')
+    {}
+
+
+    lemma Lemma_Inv_Implies_Safety(ss : SystemState)
+    requires Inv_All(ss)
+    ensures forall r1, r2 | 
+                            && r1 in ss.nodeStates
+                            && r2 in ss.nodeStates
+                            && IsHonest(ss, r1)
+                            && IsHonest(ss, r2)
+                          :: consistentBlockchains(ss.nodeStates[r1].bc, ss.nodeStates[r2].bc)
+    {}
+
+
+    // lemma LemmaBlockchainConsistency()
 }
